x86/TranslateInstrSize.v
@@ -3,6 +3,7 @@ Require Import Asm RelocProg RelocProgram.
 Require Import Hex compcert.encode.Bits Memdata Encode.
 Require Import EncDecRet BPProperty.
 Require Import TranslateInstr RelocBinDecode.
+Require Import ReloctablesgenArchi RelocProgSemanticsArchi1 ReloctablesgenproofArchi.
 Import Hex Bits.
 Import ListNotations.
 
@@ -12,7 +13,7 @@ Local Open Scope bits_scope.
 
 
 Lemma instr_eq_size: forall i1 i2,
-    instr_eq i1 i2 -> instr_size_asm i1 = instr_size_asm i2.
+    RelocBinDecode.instr_eq i1 i2 -> instr_size_asm i1 = instr_size_asm i2.
 Proof.
   Transparent instr_size_asm.
   intros. unfold instr_eq in H.
@@ -20,8 +21,6 @@ Proof.
   destruct Archi.ptr64 eqn:PTR.
   -
   destruct i1;try inv H;destruct i2;try inv H;cbn [instr_size_asm];auto.
-  (* Pmovzl and Pmov_rr: Pmov_rr depend on Ptr64 *)
-  admit.
 
   unfold rex_prefix_check_rr,rex_prefix_check_r.
   rewrite PTR. destr.
@@ -36,7 +35,163 @@ Proof.
   -
     destruct i1;try inv H;destruct i2;try inv H;cbn [instr_size_asm];auto.
     
-Admitted.
+    unfold rex_prefix_check_rr,rex_prefix_check_r.
+    rewrite PTR. auto.
+    
+    destruct H11. subst. auto.
+
+    rewrite PTR. auto.
+    rewrite PTR. auto.
+Qed.
+
+Lemma rev_id_eliminate_size: forall i id, instr_size_asm i = instr_size_asm (rev_id_eliminate id i).
+Proof.
+  destruct i;intros;cbn;auto;
+    try (destruct a;destruct const;simpl;auto).
+  try (destruct ad;destruct const;simpl;auto).
+Qed.
+
+Lemma instr_eq_size_reloc: forall i1 i2, instr_eq i1 i2 -> instr_size_asm i1 = instr_size_asm i2.
+Proof.
+  unfold instr_eq.
+  intros. destruct i1;subst;auto.
+  destruct i2;try congruence;subst;auto.
+Qed.  
+
+Lemma id_eliminate_size_unchanged:forall i, instr_size_asm i = instr_size_asm (id_eliminate i).
+Proof.
+  Transparent addrmode_size.
+  destruct i;simpl;auto;
+    try (destruct a;destruct ofs;try destruct p;destruct base;destruct const;try destruct p;simpl;auto).
+
+  try (destruct ad;destruct ofs;try destruct p;destruct base;destruct const;try destruct p;simpl;auto).
+Qed.
+  
+Lemma rex_prefix_check_r_bound: forall r,
+    0 <= rex_prefix_check_r r.
+Proof.
+  destruct r;unfold rex_prefix_check_r;destr;simpl;try lia.
+Qed.
+
+Lemma rex_prefix_check_fr_bound: forall r,
+    0 <= rex_prefix_check_fr r.
+Proof.
+  destruct r;unfold rex_prefix_check_fr;destr;simpl;try lia.
+Qed.
+
+Lemma rex_prefix_check_rr_bound: forall r1 r2,
+    0 <= rex_prefix_check_rr r1 r2.
+Proof.
+  destruct r1;destruct r2;unfold rex_prefix_check_rr;destr;simpl;try lia.
+Qed.
 
 
+Lemma rex_prefix_check_frr_bound: forall r1 r2,
+    0 <= rex_prefix_check_frr r1 r2.
+Proof.
+  destruct r1;destruct r2;unfold rex_prefix_check_frr;destr;simpl;try lia.
+Qed.
+
+
+Lemma rex_prefix_check_a_bound: forall a,
+    0 <= rex_prefix_check_a a.
+Proof.
+  Transparent addrmode_size.
+  unfold rex_prefix_check_a.
+  destruct a;destruct ofs;try destruct p;destruct base;destruct const;try destruct p;simpl;auto;
+  repeat destr;lia.
+Qed.
+
+Lemma rex_prefix_check_ra_bound: forall r a,
+    0 <= rex_prefix_check_ra r a.
+Proof.
+  Transparent addrmode_size.
+  unfold rex_prefix_check_ra.
+  destruct r;
+  destruct a;destruct ofs;try destruct p;destruct base;destruct const;try destruct p;simpl;auto;
+  repeat destr;lia.
+Qed.
+
+Lemma rex_prefix_check_fa_bound: forall r a,
+    0 <= rex_prefix_check_fa r a.
+Proof.
+  Transparent addrmode_size.
+  unfold rex_prefix_check_fa.
+  destruct r;
+  destruct a;destruct ofs;try destruct p;destruct base;destruct const;try destruct p;simpl;auto;
+  repeat destr;lia.
+Qed.
+
+Lemma addrmode_reloc_offset_bound: forall a,
+    0 < addrmode_reloc_offset a < addrmode_size a.
+Proof.
+  Transparent addrmode_size.
+  unfold addrmode_size.
+  destruct a;destruct ofs;try destruct p;destruct base;destruct const;try destruct p;simpl;lia.
+Qed.
+
+Ltac check_r :=
+  match goal with
+  | |- context [rex_prefix_check_r ?r] =>
+    generalize (rex_prefix_check_r_bound r)
+  end.
+
+Ltac check_rr :=
+  match goal with
+  | |- context [rex_prefix_check_rr ?r1 ?r2] =>
+    generalize (rex_prefix_check_rr_bound ?r1 ?r2)
+  end.
+
+Ltac check_f :=
+  match goal with
+  | |- context [rex_prefix_check_fr ?r] =>
+    generalize (rex_prefix_check_fr_bound r)
+  end.
+
+Ltac check_frr :=
+  match goal with
+  | |- context [rex_prefix_check_frr ?r1 ?r2] =>
+    generalize (rex_prefix_check_frr_bound ?r1 ?r2)
+  end.
+
+
+Ltac check_a :=
+  match goal with
+  | |- context [rex_prefix_check_a ?a] =>
+    generalize (rex_prefix_check_a_bound a)
+  end.
+
+Ltac check_ra :=
+  match goal with
+  | |- context [rex_prefix_check_ra ?r ?a] =>
+    generalize (rex_prefix_check_ra_bound r a)
+  end.
+
+Ltac check_fa :=
+  match goal with
+  | |- context [rex_prefix_check_fa ?r ?a] =>
+    generalize (rex_prefix_check_fa_bound r a)
+  end.
+
+Ltac addrmode_reloc_offset_check:=
+  match goal with
+  | |- context [addrmode_reloc_offset ?a ] =>
+    generalize (addrmode_reloc_offset_bound a)
+  end.
+
+Lemma instr_reloc_bound :
+  forall i ofs,
+    instr_reloc_offset i = OK ofs -> 0 < ofs < instr_size_asm i.
+Proof.
+  destruct i;cbn [instr_reloc_offset];cbn [instr_size_asm];intros;destr_in H;try monadInv H;    
+    try check_r;
+    try check_f;
+    try check_rr;
+    try check_frr;
+    try check_a;
+    try check_ra;
+    try check_fa;
+    try addrmode_reloc_offset_check;
+    try lia.
+Qed.
 
